lib/Unqualify.thy
@@ -1,0 +1,150 @@
+(*
+  Drop mandatory qualifiers from internal locale facts, constants and types
+  Optionally add a different qualifier
+*)
+
+theory Unqualify
+imports Main
+keywords "unqualify_facts" :: thy_decl and "unqualify_consts" :: thy_decl and "unqualify_types" :: thy_decl
+begin
+
+ML \<open>
+
+local
+
+fun map_option _ NONE = NONE
+  | map_option f (SOME x) = SOME (f x)
+
+fun make_binding_raw (nm, pos) =
+  let
+    val path = Long_Name.explode nm |> rev;
+    val b' = fold (Binding.qualify true) (tl path) (Binding.make (hd path, pos));
+  in b' end
+
+fun make_binding b =
+  let
+    val nm = Binding.name_of b;
+    val pos = Binding.pos_of b;
+  in make_binding_raw (nm, pos) end
+
+val parse_opt_target = Parse.opt_target >> 
+  (map_option (apfst (fn raw_nm =>
+          case try (unprefix "$") raw_nm of SOME nm' => getenv_strict nm' | NONE => raw_nm)))
+
+val unqualify_parse = parse_opt_target -- Scan.option (Args.parens Parse.name) -- Scan.repeat1 Parse.binding
+
+in
+
+val _ =
+  Outer_Syntax.command @{command_keyword unqualify_facts} "unqualify facts"
+    (unqualify_parse >> (fn ((target,qual),bs) =>
+      Toplevel.local_theory NONE target (fn lthy =>
+      let                            
+        val facts = Proof_Context.facts_of lthy;
+
+        fun retrieve b = Facts.retrieve (Context.Proof lthy) facts (Binding.name_of b, Binding.pos_of b);
+
+
+        val thmss = map (`retrieve) bs
+          |> map (fn ({thms, ...}, b) => (make_binding b, thms));
+
+        val lthy' = Local_Theory.background_theory (fn thy =>
+          let
+            val naming = the_default I (map_option Name_Space.mandatory_path qual) Name_Space.global_naming;
+            val thy' = Context.theory_map (Name_Space.map_naming (K naming)) thy;
+            val export = Morphism.fact (Local_Theory.standard_morphism lthy (Proof_Context.init_global thy));
+          in
+            fold (fn (b, thms) => Global_Theory.store_thms (b,export thms) #> snd) thmss thy'
+          end) lthy
+
+       in
+       lthy'
+       end)))
+
+val k = Parse.for_fixes
+
+
+val _ =
+  Outer_Syntax.command @{command_keyword unqualify_consts} "unqualify consts"
+    (parse_opt_target -- Scan.option (Args.parens Parse.name) -- 
+      Scan.repeat1 (Parse.position Parse.term) >> (fn ((target,qual),bs) =>
+      Toplevel.local_theory NONE target (fn lthy =>
+      let
+
+        val ts = map (`(Syntax.parse_term lthy o fst)) bs;
+
+        fun get_const 
+            (( t as Const ("_type_constraint_", _) $
+                (Const ("_type_constraint_", _) $
+                  Const (nm, _))), (_, pos)) = ((nm, pos), t)
+           | get_const (t as (Const ("_type_constraint_", _) $
+                  Const (nm, _)), (_, pos)) = ((nm, pos), t)
+           | get_const (t, (_,pos)) = error ("Not a constant or abbreviation: " ^ Syntax.string_of_term lthy t ^ Position.here pos)
+
+        val ts' = map (apsnd (Syntax.check_term lthy) o apfst make_binding_raw o get_const) ts;
+
+        val lthy' = Local_Theory.background_theory (fn thy =>
+          let
+            val naming = the_default I (map_option Name_Space.mandatory_path qual) Name_Space.global_naming;
+            val thy' = Context.theory_map (Name_Space.map_naming (K naming)) thy;
+            val export = Morphism.term (Local_Theory.standard_morphism lthy (Proof_Context.init_global thy));
+  
+          in
+            fold (fn (b, t) =>
+              let
+                val b' = make_binding b;
+                val nm = Binding.name_of b';
+              in
+               Sign.add_abbrev nm (b', export t) #> snd
+              end) ts' thy'
+          end) lthy
+
+       in
+       lthy'
+       end)))
+
+
+val _ =
+  Outer_Syntax.command @{command_keyword unqualify_types} "unqualify types"
+    (parse_opt_target -- Scan.option (Args.parens Parse.name) -- 
+      Scan.repeat1 (Parse.position Parse.typ) >> (fn ((target,qual),bs) =>
+      Toplevel.local_theory NONE target (fn lthy =>
+      let
+        
+        fun err (T, pos) = 
+          error ("Not a defined type or type synonym: " ^ Syntax.string_of_typ lthy T ^ Position.here pos)
+
+   
+        val Ts = map (`(Syntax.parse_typ lthy o fst)) bs;
+
+        fun get_type (T, (_, pos)) = case try dest_Type T of
+        SOME (nm, Ts) => (if can dest_funT T then err (T,pos) else ((nm, pos), (T,Ts)))
+        | NONE => err (T,pos)
+
+        fun check_Ts (T,Ts) = (Syntax.check_typ lthy T, 
+          fold Term.add_tfree_namesT Ts [])
+
+        val Ts' = map (apsnd check_Ts o apfst make_binding_raw o get_type) Ts;
+
+        val lthy' = Local_Theory.background_theory (fn thy =>
+          let
+            val naming = the_default I (map_option Name_Space.mandatory_path qual) Name_Space.global_naming;
+            val thy' = Context.theory_map (Name_Space.map_naming (K naming)) thy;
+          in
+            fold (fn (b, (T,frees)) =>
+              let
+                val b' = make_binding b;
+              in
+               Sign.add_type_abbrev lthy (b',frees, T)
+              end) Ts' thy'
+          end) lthy
+
+       in
+       lthy'
+       end)))
+
+end
+
+\<close>
+
+end
