proof/invariant-abstract/ARM/ArchInvariants_AI.thy
@@ -1,0 +1,867 @@
+(*
+ * Copyright 2014, General Dynamics C4 Systems
+ *
+ * This software may be distributed and modified according to the terms of
+ * the GNU General Public License version 2. Note that NO WARRANTY is provided.
+ * See "LICENSE_GPLv2.txt" for details.
+ *
+ * @TAG(GD_GPL)
+ *)
+
+theory ArchInvariants_AI
+imports "../LevityCatch_AI"
+begin
+
+section "Move this up"
+
+qualify ARM
+
+-- ---------------------------------------------------------------------------
+section "Things to Move Up"
+
+(* FIXME: move to spec level *)
+(* global data and code of the kernel, not covered by any cap *)
+axiomatization
+  kernel_data_refs :: "word32 set"
+
+end_qualify
+
+-- ---------------------------------------------------------------------------
+section "ARM-specific invariant definitions"
+
+context ARM begin
+
+lemmas aa_type_simps =
+  aa_type_def[split_simps arch_kernel_obj.split]
+
+
+definition
+  aobj_at :: "(arch_kernel_obj \<Rightarrow> bool) \<Rightarrow> obj_ref \<Rightarrow> 'z::state_ext state \<Rightarrow> bool"
+where
+  "aobj_at P ref s \<equiv> \<exists>ko. kheap s ref = Some (ArchObj ko) \<and> P ko"
+
+abbreviation
+  "ako_at k \<equiv> aobj_at (op = k)"
+
+definition
+  "vmsz_aligned ref sz \<equiv> is_aligned ref (pageBitsForSize sz)"
+
+definition
+  "wellformed_mapdata sz \<equiv>
+   \<lambda>(asid, vref). 0 < asid \<and> asid \<le> 2^asid_bits - 1
+                \<and> vmsz_aligned vref sz \<and> vref < kernel_base"
+
+definition
+  wellformed_acap :: "arch_cap \<Rightarrow> bool"
+where
+  "wellformed_acap ac \<equiv>
+   case ac of
+     Arch_Structs_A.ASIDPoolCap r as
+       \<Rightarrow> is_aligned as asid_low_bits \<and> as \<le> 2^asid_bits - 1
+   | Arch_Structs_A.PageCap r rghts sz mapdata \<Rightarrow> rghts \<in> valid_vm_rights \<and>
+     case_option True (wellformed_mapdata sz) mapdata
+   | Arch_Structs_A.PageTableCap r (Some mapdata) \<Rightarrow>
+     wellformed_mapdata ARMSection mapdata
+   | Arch_Structs_A.PageDirectoryCap r (Some asid) \<Rightarrow>
+     0 < asid \<and> asid \<le> 2^asid_bits - 1
+   | _ \<Rightarrow> True"
+
+lemmas wellformed_acap_simps =
+  wellformed_mapdata_def wellformed_acap_def[split_simps arch_cap.split]
+
+abbreviation
+  "atyp_at T \<equiv> aobj_at (\<lambda>ob. aa_type ob = T)"
+
+(* this time with typ_at. might lead to confusion, but this is how
+   the rest should have been defined.. *)
+abbreviation
+  "asid_pool_at \<equiv> atyp_at AASIDPool"
+abbreviation
+  "page_table_at \<equiv> atyp_at APageTable"
+abbreviation
+  "page_directory_at \<equiv> atyp_at APageDirectory"
+
+definition
+  "pde_at p \<equiv> page_directory_at (p && ~~ mask pd_bits)
+                  and K (is_aligned p 2)"
+definition
+  "pte_at p \<equiv> page_table_at (p && ~~ mask pt_bits)
+                  and K (is_aligned p 2)"
+
+definition
+  valid_arch_cap_ref :: "arch_cap \<Rightarrow> 'z::state_ext state \<Rightarrow> bool"
+where
+  "valid_arch_cap_ref ac s \<equiv> (case ac of
+    Arch_Structs_A.ASIDPoolCap r as \<Rightarrow> atyp_at AASIDPool r s
+  | Arch_Structs_A.ASIDControlCap \<Rightarrow> True
+  | Arch_Structs_A.PageCap r rghts sz mapdata \<Rightarrow> atyp_at (AIntData sz) r s
+  | Arch_Structs_A.PageTableCap r mapdata \<Rightarrow> atyp_at APageTable r s
+  | Arch_Structs_A.PageDirectoryCap r mapdata\<Rightarrow> atyp_at APageDirectory r s)"
+
+lemmas valid_arch_cap_ref_simps =
+  valid_arch_cap_ref_def[split_simps arch_cap.split]
+
+definition
+  valid_arch_cap :: "arch_cap \<Rightarrow> 'z::state_ext state \<Rightarrow> bool"
+where
+  "valid_arch_cap ac s \<equiv> (case ac of
+    Arch_Structs_A.ASIDPoolCap r as \<Rightarrow>
+         atyp_at AASIDPool r s \<and> is_aligned as asid_low_bits
+           \<and> as \<le> 2^asid_bits - 1
+  | Arch_Structs_A.ASIDControlCap \<Rightarrow> True
+  | Arch_Structs_A.PageCap r rghts sz mapdata \<Rightarrow>
+    atyp_at (AIntData sz) r s \<and> rghts \<in> valid_vm_rights \<and>
+    (case mapdata of None \<Rightarrow> True | Some (asid, ref) \<Rightarrow> 0 < asid \<and> asid \<le> 2^asid_bits - 1
+                                             \<and> vmsz_aligned ref sz \<and> ref < kernel_base)
+  | Arch_Structs_A.PageTableCap r mapdata \<Rightarrow>
+    atyp_at APageTable r s \<and>
+    (case mapdata of None \<Rightarrow> True
+       | Some (asid, vref) \<Rightarrow> 0 < asid \<and> asid \<le> 2 ^ asid_bits - 1
+                                \<and> vref < kernel_base
+                                \<and> is_aligned vref (pageBitsForSize ARMSection))
+  | Arch_Structs_A.PageDirectoryCap r mapdata \<Rightarrow>
+    atyp_at APageDirectory r s \<and>
+    case_option True (\<lambda>asid. 0 < asid \<and> asid \<le> 2^asid_bits - 1) mapdata)"
+
+lemmas valid_arch_cap_simps =
+  valid_arch_cap_def[split_simps arch_cap.split]
+
+primrec
+  acap_class :: "arch_cap \<Rightarrow> capclass"
+where
+  "acap_class (arch_cap.ASIDPoolCap x y)      = PhysicalClass"
+| "acap_class (arch_cap.ASIDControlCap)       = ASIDMasterClass"
+| "acap_class (arch_cap.PageCap x y sz z)     = PhysicalClass"
+| "acap_class (arch_cap.PageTableCap x y)     = PhysicalClass"
+| "acap_class (arch_cap.PageDirectoryCap x y) = PhysicalClass"
+
+definition
+  valid_ipc_buffer_cap :: "cap \<Rightarrow> word32 \<Rightarrow> bool"
+where
+  "valid_ipc_buffer_cap c bufptr \<equiv>
+         case c of
+              cap.ArchObjectCap (arch_cap.PageCap ref rghts sz mapdata) \<Rightarrow>
+                   is_aligned bufptr msg_align_bits
+
+            | _ \<Rightarrow> True"
+
+primrec
+  valid_pte :: "Arch_Structs_A.pte \<Rightarrow> 'z::state_ext state \<Rightarrow> bool"
+where
+  "valid_pte (Arch_Structs_A.InvalidPTE) = \<top>"
+| "valid_pte (Arch_Structs_A.LargePagePTE ptr x y) =
+   (\<lambda>s. is_aligned ptr pageBits \<and>
+        atyp_at (AIntData ARMLargePage) (Platform.ptrFromPAddr ptr) s)"
+| "valid_pte (Arch_Structs_A.SmallPagePTE ptr x y) =
+   (\<lambda>s. is_aligned ptr pageBits \<and>
+        atyp_at (AIntData ARMSmallPage) (Platform.ptrFromPAddr ptr) s)"
+
+primrec
+  valid_pde :: "Arch_Structs_A.pde \<Rightarrow> 'z::state_ext state \<Rightarrow> bool"
+where
+  "valid_pde (Arch_Structs_A.InvalidPDE) = \<top>"
+| "valid_pde (Arch_Structs_A.SectionPDE ptr x y z) =
+   (\<lambda>s. is_aligned ptr pageBits \<and>
+        atyp_at (AIntData ARMSection) (Platform.ptrFromPAddr ptr) s)"
+| "valid_pde (Arch_Structs_A.SuperSectionPDE ptr x z) =
+   (\<lambda>s. is_aligned ptr pageBits \<and>
+        atyp_at (AIntData ARMSuperSection)
+               (Platform.ptrFromPAddr ptr) s)"
+| "valid_pde (Arch_Structs_A.PageTablePDE ptr x z) =
+   (atyp_at APageTable (Platform.ptrFromPAddr ptr))"
+
+
+definition
+  kernel_mapping_slots :: "12 word set" where
+ "kernel_mapping_slots \<equiv> {x. x \<ge> ucast (kernel_base >> 20)}"
+
+primrec
+  valid_arch_obj :: "arch_kernel_obj \<Rightarrow> 'z::state_ext state \<Rightarrow> bool"
+where
+  "valid_arch_obj (Arch_Structs_A.ASIDPool pool) =
+   (\<lambda>s. \<forall>x \<in> ran pool. atyp_at  APageDirectory x s)"
+| "valid_arch_obj (Arch_Structs_A.PageDirectory pd) =
+   (\<lambda>s. \<forall>x \<in> -kernel_mapping_slots. valid_pde (pd x) s)"
+| "valid_arch_obj (Arch_Structs_A.PageTable pt) = (\<lambda>s. \<forall>x. valid_pte (pt x) s)"
+| "valid_arch_obj (DataPage sz) = \<top>"
+
+definition
+  wellformed_pte :: "Arch_Structs_A.pte \<Rightarrow> bool"
+where
+  "wellformed_pte pte \<equiv> case pte of
+     Arch_Structs_A.pte.LargePagePTE p attr r \<Rightarrow>
+       ParityEnabled \<notin> attr \<and> r \<in> valid_vm_rights
+   | Arch_Structs_A.pte.SmallPagePTE p attr r \<Rightarrow>
+       ParityEnabled \<notin> attr \<and> r \<in> valid_vm_rights
+   | _ \<Rightarrow> True"
+
+definition
+  wellformed_pde :: "Arch_Structs_A.pde \<Rightarrow> bool"
+where
+  "wellformed_pde pde \<equiv> case pde of
+     Arch_Structs_A.pde.PageTablePDE p attr mw \<Rightarrow> attr \<subseteq> {ParityEnabled}
+   | Arch_Structs_A.pde.SectionPDE p attr mw r \<Rightarrow> r \<in> valid_vm_rights
+   | Arch_Structs_A.pde.SuperSectionPDE p attr r \<Rightarrow> r \<in> valid_vm_rights
+   | _ \<Rightarrow> True"
+
+definition
+  wellformed_arch_obj :: "arch_kernel_obj \<Rightarrow> bool"
+where
+  "wellformed_arch_obj ao \<equiv> case ao of
+     PageTable pt \<Rightarrow> (\<forall>pte\<in>range pt. wellformed_pte pte)
+   | PageDirectory pd \<Rightarrow> (\<forall>pde\<in>range pd. wellformed_pde pde)
+   | _ \<Rightarrow> True"
+
+section "Virtual Memory"
+
+definition
+  equal_kernel_mappings :: "'z::state_ext state \<Rightarrow> bool"
+where
+ "equal_kernel_mappings \<equiv> \<lambda>s.
+    \<forall>x y pd pd'. ako_at (PageDirectory pd) x s
+         \<and> ako_at (PageDirectory pd') y s
+       \<longrightarrow> (\<forall>w \<in> kernel_mapping_slots. pd w = pd' w)"
+
+definition
+  pde_ref :: "Arch_Structs_A.pde \<Rightarrow> obj_ref option"
+where
+  "pde_ref pde \<equiv> case pde of
+    Arch_Structs_A.PageTablePDE ptr x z \<Rightarrow> Some (Platform.ptrFromPAddr ptr)
+  | _ \<Rightarrow> None"
+
+datatype vs_ref = VSRef word32 "aa_type option"
+
+definition
+  vs_ref_atype :: "vs_ref \<Rightarrow> aa_type option" where
+ "vs_ref_atype vsref \<equiv> case vsref of VSRef x atype \<Rightarrow> atype"
+
+definition
+  vs_refs :: "arch_kernel_obj \<Rightarrow> (vs_ref \<times> obj_ref) set" where
+  "vs_refs \<equiv> \<lambda>ko. case ko of
+    (Arch_Structs_A.ASIDPool pool) \<Rightarrow>
+      (\<lambda>(r,p). (VSRef (ucast r) (Some AASIDPool), p)) ` graph_of pool
+  | (Arch_Structs_A.PageDirectory pd) \<Rightarrow>
+      (\<lambda>(r,p). (VSRef (ucast r) (Some APageDirectory), p)) `
+      graph_of (\<lambda>x. if x \<in> kernel_mapping_slots then None else pde_ref (pd x))
+  | _ \<Rightarrow> {}"
+
+type_synonym vs_chain = "vs_ref list \<times> obj_ref"
+type_synonym 'a rel = "('a \<times> 'a) set"
+
+definition
+  vs_lookup1 :: "'z::state_ext state \<Rightarrow> vs_chain rel" where
+  "vs_lookup1 s \<equiv> {((rs,p),(rs',p')). \<exists>ko r. ako_at ko p s
+                                      \<and> rs' = (r # rs)
+                                      \<and> (r, p') \<in> vs_refs ko}"
+
+abbreviation (input)
+  vs_lookup_trans :: "'z::state_ext state \<Rightarrow> vs_chain rel" where
+  "vs_lookup_trans s \<equiv> (vs_lookup1 s)^*"
+
+abbreviation
+  vs_lookup1_abbr :: "vs_chain \<Rightarrow> vs_chain \<Rightarrow> 'z::state_ext state \<Rightarrow> bool"
+  ("_ \<rhd>1 _" [80,80] 81) where
+  "ref \<rhd>1 ref' \<equiv> \<lambda>s. (ref,ref') \<in> vs_lookup1 s"
+
+abbreviation
+  vs_lookup_trans_abbr :: "vs_chain \<Rightarrow> vs_chain \<Rightarrow> 'z::state_ext state \<Rightarrow> bool"
+  ("_ \<rhd>* _" [80,80] 81) where
+  "ref \<rhd>* ref' \<equiv> \<lambda>s. (ref,ref') \<in> vs_lookup_trans s"
+
+definition
+  vs_asid_refs :: "(word8 \<rightharpoonup> obj_ref) \<Rightarrow> vs_chain set"
+where
+  "vs_asid_refs t \<equiv> (\<lambda>(r,p). ([VSRef (ucast r) None], p)) ` graph_of t"
+
+definition
+  vs_lookup :: "'z::state_ext state \<Rightarrow> vs_chain set"
+where
+  "vs_lookup \<equiv> \<lambda>s. vs_lookup_trans s `` vs_asid_refs (arm_asid_table (arch_state s))"
+
+abbreviation
+  vs_lookup_abbr :: "vs_ref list \<Rightarrow> obj_ref \<Rightarrow> 'z::state_ext state \<Rightarrow> bool"
+  ("_ \<rhd> _" [80,80] 81) where
+  "rs \<rhd> p \<equiv> \<lambda>s. (rs,p) \<in> vs_lookup s"
+
+abbreviation
+  is_reachable_abbr :: "obj_ref \<Rightarrow> 'z::state_ext state \<Rightarrow> bool" ("\<exists>\<rhd> _" [80] 81) where
+  "\<exists>\<rhd> p \<equiv> \<lambda>s. \<exists>ref. (ref \<rhd> p) s"
+
+definition
+  valid_arch_objs :: "'z::state_ext state \<Rightarrow> bool"
+where
+  "valid_arch_objs \<equiv> \<lambda>s. \<forall>p rs ao. (rs \<rhd> p) s \<longrightarrow> ako_at ao p s \<longrightarrow> valid_arch_obj ao s"
+
+definition
+  pde_ref_pages :: "Arch_Structs_A.pde \<Rightarrow> obj_ref option"
+where
+  "pde_ref_pages pde \<equiv> case pde of
+    Arch_Structs_A.PageTablePDE ptr x z \<Rightarrow> Some (Platform.ptrFromPAddr ptr)
+  | Arch_Structs_A.SectionPDE ptr x y z \<Rightarrow> Some (Platform.ptrFromPAddr ptr)
+  | Arch_Structs_A.SuperSectionPDE ptr x z \<Rightarrow> Some (Platform.ptrFromPAddr ptr)
+  | _ \<Rightarrow> None"
+
+definition
+  pte_ref_pages :: "Arch_Structs_A.pte \<Rightarrow> obj_ref option"
+where
+  "pte_ref_pages pte \<equiv> case pte of
+    Arch_Structs_A.SmallPagePTE ptr x z \<Rightarrow> Some (Platform.ptrFromPAddr ptr)
+  | Arch_Structs_A.LargePagePTE ptr x z \<Rightarrow> Some (Platform.ptrFromPAddr ptr)
+  | _ \<Rightarrow> None"
+
+definition
+  vs_refs_pages :: "arch_kernel_obj \<Rightarrow> (vs_ref \<times> obj_ref) set" where
+  "vs_refs_pages \<equiv> \<lambda>ko. case ko of
+    (Arch_Structs_A.ASIDPool pool) \<Rightarrow>
+      (\<lambda>(r,p). (VSRef (ucast r) (Some AASIDPool), p)) ` graph_of pool
+  | (Arch_Structs_A.PageDirectory pd) \<Rightarrow>
+      (\<lambda>(r,p). (VSRef (ucast r) (Some APageDirectory), p)) `
+      graph_of (\<lambda>x. if x \<in> kernel_mapping_slots then None else pde_ref_pages (pd x))
+  | (Arch_Structs_A.PageTable pt) \<Rightarrow>
+      (\<lambda>(r,p). (VSRef (ucast r) (Some APageTable), p)) `
+      graph_of (pte_ref_pages o pt)
+  | _ \<Rightarrow> {}"
+
+definition
+  vs_lookup_pages1 :: "'z :: state_ext state \<Rightarrow> vs_chain rel" where
+  "vs_lookup_pages1 s \<equiv> {((rs,p),(rs',p')). \<exists>ko r. ako_at ko p s
+                                          \<and> rs' = (r # rs)
+                                          \<and> (r, p') \<in> vs_refs_pages ko}"
+
+abbreviation (input)
+  vs_lookup_pages_trans :: "'z :: state_ext state \<Rightarrow> vs_chain rel" where
+  "vs_lookup_pages_trans s \<equiv> (vs_lookup_pages1 s)^*"
+
+abbreviation
+  vs_lookup_pages1_abbr :: "vs_chain \<Rightarrow> vs_chain \<Rightarrow> 'z :: state_ext state \<Rightarrow> bool"
+  ("_ \<unrhd>1 _" [80,80] 81) where
+  "ref \<unrhd>1 ref' \<equiv> \<lambda>s. (ref,ref') \<in> vs_lookup_pages1 s"
+
+abbreviation
+  vs_lookup_pages_trans_abbr :: "vs_chain \<Rightarrow> vs_chain \<Rightarrow> 'z :: state_ext state \<Rightarrow> bool"
+  ("_ \<unrhd>* _" [80,80] 81) where
+  "ref \<unrhd>* ref' \<equiv> \<lambda>s. (ref,ref') \<in> vs_lookup_pages_trans s"
+
+definition
+  vs_lookup_pages :: "'z ::state_ext state \<Rightarrow> vs_chain set"
+where
+  "vs_lookup_pages \<equiv> \<lambda>s. vs_lookup_pages_trans s `` vs_asid_refs (arm_asid_table (arch_state s))"
+
+abbreviation
+  vs_lookup_pages_abbr :: "vs_ref list \<Rightarrow> obj_ref \<Rightarrow> 'z :: state_ext state \<Rightarrow> bool"
+  ("_ \<unrhd> _" [80,80] 81) where
+  "rs \<unrhd> p \<equiv> \<lambda>s. (rs,p) \<in> vs_lookup_pages s"
+
+abbreviation
+  is_reachable_pages_abbr :: "obj_ref \<Rightarrow> 'z :: state_ext state \<Rightarrow> bool" ("\<exists>\<unrhd> _" [80] 81) where
+  "\<exists>\<unrhd> p \<equiv> \<lambda>s. \<exists>ref. (ref \<unrhd> p) s"
+
+definition
+  pde_mapping_bits :: "nat"
+where
+ "pde_mapping_bits \<equiv> pageBitsForSize ARMSection"
+
+definition
+  pte_mapping_bits :: "nat"
+where
+ "pte_mapping_bits \<equiv> pageBitsForSize ARMSmallPage"
+
+definition
+  valid_pte_kernel_mappings :: "Arch_Structs_A.pte \<Rightarrow> vspace_ref
+                                   \<Rightarrow> arm_vspace_region_uses \<Rightarrow> bool"
+where
+ "valid_pte_kernel_mappings pte vref uses \<equiv> case pte of
+    Arch_Structs_A.InvalidPTE \<Rightarrow>
+        \<forall>x \<in> {vref .. vref + 2 ^ pte_mapping_bits - 1}.
+                    uses x \<noteq> ArmVSpaceKernelWindow
+  | Arch_Structs_A.SmallPagePTE ptr atts rghts \<Rightarrow>
+        Platform.ptrFromPAddr ptr = vref
+        \<and> (\<exists>use. (\<forall>x \<in> {vref .. vref + 2 ^ pte_mapping_bits - 1}. uses x = use)
+             \<and> (use = ArmVSpaceKernelWindow
+                    \<or> use = ArmVSpaceDeviceWindow))
+        \<and> rghts = {}
+  | Arch_Structs_A.LargePagePTE ptr atts rghts \<Rightarrow>
+        Platform.ptrFromPAddr ptr = (vref && ~~ mask (pageBitsForSize ARMLargePage))
+        \<and> (\<exists>use. (\<forall>x \<in> {vref .. vref + 2 ^ pte_mapping_bits - 1}. uses x = use)
+             \<and> (use = ArmVSpaceKernelWindow
+                    \<or> use = ArmVSpaceDeviceWindow))
+        \<and> rghts = {}"
+
+definition
+  valid_pt_kernel_mappings :: "vspace_ref \<Rightarrow> arm_vspace_region_uses \<Rightarrow> arch_kernel_obj \<Rightarrow> bool"
+where
+ "valid_pt_kernel_mappings vref uses obj \<equiv> case obj of
+    PageTable pt \<Rightarrow>
+        \<forall>x. valid_pte_kernel_mappings
+             (pt x) (vref + (ucast x << pte_mapping_bits)) uses
+  | _ \<Rightarrow> False"
+
+definition
+  valid_pde_kernel_mappings :: "Arch_Structs_A.pde \<Rightarrow> vspace_ref \<Rightarrow> arm_vspace_region_uses \<Rightarrow> 'z::state_ext state \<Rightarrow> bool"
+where
+ "valid_pde_kernel_mappings pde vref uses \<equiv> case pde of
+    Arch_Structs_A.InvalidPDE \<Rightarrow>
+        (\<lambda>s. \<forall>x \<in> {vref .. vref + 2 ^ pde_mapping_bits - 1}.
+                    uses x \<noteq> ArmVSpaceKernelWindow)
+  | Arch_Structs_A.PageTablePDE ptr _ _ \<Rightarrow>
+        aobj_at (valid_pt_kernel_mappings vref uses)
+                    (Platform.ptrFromPAddr ptr)
+  | Arch_Structs_A.SectionPDE ptr atts _ rghts \<Rightarrow>
+        (\<lambda>s. Platform.ptrFromPAddr ptr = vref
+             \<and> (\<exists>use. (\<forall>x \<in> {vref .. vref + 2 ^ pde_mapping_bits - 1}. uses x = use)
+                   \<and> (use = ArmVSpaceKernelWindow
+                            \<or> use = ArmVSpaceDeviceWindow))
+             \<and> rghts = {})
+  | Arch_Structs_A.SuperSectionPDE ptr atts rghts \<Rightarrow>
+        (\<lambda>s. Platform.ptrFromPAddr ptr = (vref && ~~ mask (pageBitsForSize ARMSuperSection))
+             \<and> (\<forall>x \<in> {vref .. vref + 2 ^ pde_mapping_bits - 1}.
+                   uses x = ArmVSpaceKernelWindow)
+             \<and> rghts = {})"
+
+definition
+  valid_pd_kernel_mappings :: "arm_vspace_region_uses \<Rightarrow> 'z::state_ext state
+                                    \<Rightarrow> arch_kernel_obj \<Rightarrow> bool"
+where
+ "valid_pd_kernel_mappings uses \<equiv> \<lambda>s obj.
+  case obj of
+    PageDirectory pd \<Rightarrow>
+      (\<forall>x. valid_pde_kernel_mappings
+             (pd x) (ucast x << pde_mapping_bits) uses s)
+  | _ \<Rightarrow> False"
+
+definition
+  valid_global_pd_mappings :: "'z::state_ext state \<Rightarrow> bool"
+where
+ "valid_global_pd_mappings \<equiv> \<lambda>s.
+  aobj_at (valid_pd_kernel_mappings (arm_kernel_vspace (arch_state s)) s)
+    (arm_global_pd (arch_state s)) s"
+
+definition
+  valid_ao_at :: "obj_ref \<Rightarrow> 'z::state_ext state \<Rightarrow> bool"
+where
+  "valid_ao_at p \<equiv> \<lambda>s. \<exists>ao. ako_at ao p s \<and> valid_arch_obj ao s"
+
+definition
+  "valid_pde_mappings pde \<equiv> case pde of
+    Arch_Structs_A.SectionPDE ptr _ _ _ \<Rightarrow> is_aligned ptr pageBits
+  | Arch_Structs_A.SuperSectionPDE ptr _ _ \<Rightarrow> is_aligned ptr pageBits
+  | _ \<Rightarrow> True"
+
+definition
+  "empty_table S ko \<equiv>
+   case ko of
+     Arch_Structs_A.PageDirectory pd \<Rightarrow>
+       \<forall>x. (\<forall>r. pde_ref (pd x) = Some r \<longrightarrow> r \<in> S) \<and>
+            valid_pde_mappings (pd x) \<and>
+            (x \<notin> kernel_mapping_slots \<longrightarrow> pd x = Arch_Structs_A.InvalidPDE)
+   | Arch_Structs_A.PageTable pt \<Rightarrow>
+         pt = (\<lambda>x. Arch_Structs_A.InvalidPTE)
+   | _ \<Rightarrow> False"
+
+definition
+  "valid_kernel_mappings_if_pd S ko \<equiv> case ko of
+    ArchObj (Arch_Structs_A.PageDirectory pd) \<Rightarrow>
+        \<forall>x r. pde_ref (pd x) = Some r
+                  \<longrightarrow> ((r \<in> S) = (x \<in> kernel_mapping_slots))
+  | _ \<Rightarrow> True"
+
+definition
+  "aligned_pte pte \<equiv>
+     case pte of
+       Arch_Structs_A.LargePagePTE p _ _ \<Rightarrow> vmsz_aligned p ARMLargePage
+     | Arch_Structs_A.SmallPagePTE p _ _ \<Rightarrow> vmsz_aligned p ARMSmallPage
+     | _ \<Rightarrow> True"
+
+lemmas aligned_pte_simps[simp] =
+       aligned_pte_def[split_simps Arch_Structs_A.pte.split]
+
+
+definition
+  valid_global_objs :: "'z::state_ext state \<Rightarrow> bool"
+where
+  "valid_global_objs \<equiv>
+  \<lambda>s. valid_ao_at (arm_global_pd (arch_state s)) s \<and>
+           aobj_at (empty_table (set (arm_global_pts (arch_state s))))
+                  (arm_global_pd (arch_state s)) s \<and>
+      (\<forall>p\<in>set (arm_global_pts (arch_state s)).
+          \<exists>pt. ako_at (PageTable pt) p s \<and> (\<forall>x. aligned_pte (pt x)))"
+
+definition
+  valid_asid_table :: "(word8 \<rightharpoonup> obj_ref) \<Rightarrow> 'z::state_ext state \<Rightarrow> bool"
+where
+  "valid_asid_table table \<equiv> \<lambda>s. (\<forall>p \<in> ran table. asid_pool_at p s) \<and>
+                                inj_on table (dom table)"
+
+definition
+  valid_global_pts :: "'z :: state_ext state \<Rightarrow> bool"
+where
+  "valid_global_pts \<equiv> \<lambda>s.
+   \<forall>p \<in> set (arm_global_pts (arch_state s)). atyp_at APageTable p s"
+(* this property now follows from valid_global_objs:
+   "valid_global_objs s \<Longrightarrow> valid_global_pts s" *)
+
+definition
+  valid_arch_state :: "'z::state_ext state \<Rightarrow> bool"
+where
+  "valid_arch_state \<equiv> \<lambda>s.
+  atyp_at (AIntData ARMSmallPage) (arm_globals_frame (arch_state s)) s \<and>
+  valid_asid_table (arm_asid_table (arch_state s)) s \<and>
+  page_directory_at (arm_global_pd (arch_state s)) s \<and>
+  valid_global_pts s \<and>
+  is_inv (arm_hwasid_table (arch_state s))
+             (option_map fst o arm_asid_map (arch_state s))"
+
+definition
+  vs_cap_ref :: "arch_cap \<Rightarrow> vs_ref list option"
+where
+  "vs_cap_ref cap \<equiv> case cap of
+   Arch_Structs_A.ASIDPoolCap _ asid \<Rightarrow>
+     Some [VSRef (ucast (asid_high_bits_of asid)) None]
+ | Arch_Structs_A.PageDirectoryCap _ (Some asid) \<Rightarrow>
+     Some [VSRef (asid && mask asid_low_bits) (Some AASIDPool),
+           VSRef (ucast (asid_high_bits_of asid)) None]
+ | Arch_Structs_A.PageTableCap _ (Some (asid, vptr)) \<Rightarrow>
+     Some [VSRef (vptr >> 20) (Some APageDirectory),
+           VSRef (asid && mask asid_low_bits) (Some AASIDPool),
+           VSRef (ucast (asid_high_bits_of asid)) None]
+ | Arch_Structs_A.PageCap word rights ARMSmallPage (Some (asid, vptr)) \<Rightarrow>
+     Some [VSRef ((vptr >> 12) && mask 8) (Some APageTable),
+           VSRef (vptr >> 20) (Some APageDirectory),
+           VSRef (asid && mask asid_low_bits) (Some AASIDPool),
+           VSRef (ucast (asid_high_bits_of asid)) None]
+ | Arch_Structs_A.PageCap word rights ARMLargePage (Some (asid, vptr)) \<Rightarrow>
+     Some [VSRef ((vptr >> 12) && mask 8) (Some APageTable),
+           VSRef (vptr >> 20) (Some APageDirectory),
+           VSRef (asid && mask asid_low_bits) (Some AASIDPool),
+           VSRef (ucast (asid_high_bits_of asid)) None]
+ | Arch_Structs_A.PageCap word rights ARMSection (Some (asid, vptr)) \<Rightarrow>
+     Some [VSRef (vptr >> 20) (Some APageDirectory),
+           VSRef (asid && mask asid_low_bits) (Some AASIDPool),
+           VSRef (ucast (asid_high_bits_of asid)) None]
+ | Arch_Structs_A.PageCap word rights ARMSuperSection (Some (asid, vptr)) \<Rightarrow>
+     Some [VSRef (vptr >> 20) (Some APageDirectory),
+           VSRef (asid && mask asid_low_bits) (Some AASIDPool),
+           VSRef (ucast (asid_high_bits_of asid)) None]
+ | _ \<Rightarrow> None"
+
+definition
+  "is_pg_cap cap \<equiv> \<exists>p R sz m. cap =
+   arch_cap.PageCap p R sz m"
+
+definition
+  "is_pd_cap c \<equiv>
+   \<exists>p asid. c = arch_cap.PageDirectoryCap p asid"
+
+definition
+  "is_pt_cap c \<equiv> \<exists>p asid. c = arch_cap.PageTableCap p asid"
+
+definition
+  "cap_asid cap \<equiv> case cap of
+    Arch_Structs_A.PageCap _ _ _ (Some (asid, _)) \<Rightarrow> Some asid
+  | Arch_Structs_A.PageTableCap _ (Some (asid, _)) \<Rightarrow> Some asid
+  | Arch_Structs_A.PageDirectoryCap _ (Some asid) \<Rightarrow> Some asid
+  | _ \<Rightarrow> None"
+
+definition
+  arch_caps_of_state :: "'z::state_ext state \<Rightarrow> cslot_ptr \<Rightarrow> arch_cap option"
+where
+ "arch_caps_of_state s \<equiv> (\<lambda>p. if (\<exists>acap. fst (get_cap p s) = {(ArchObjectCap acap, s)})
+                         then Some (THE acap. fst (get_cap p s) = {(ArchObjectCap acap, s)})
+                         else None)"
+
+  (* needed for retype: if reachable, then cap, if cap then protected by untyped cap.
+     strengthened for preservation in cap delete: ref in cap must unmap the right objects *)
+definition
+  "valid_vs_lookup \<equiv> \<lambda>s. \<forall>p ref. (ref \<unrhd> p) s \<longrightarrow>
+  ref \<noteq> [VSRef 0 (Some AASIDPool), VSRef 0 None] \<and>
+  (\<exists>p' acap. arch_caps_of_state s p' = Some acap \<and>
+            aobj_ref acap = Some p \<and> vs_cap_ref acap = Some ref)"
+
+definition
+  global_refs :: "'z::state_ext state \<Rightarrow> obj_ref set"
+where
+  "global_refs \<equiv> \<lambda>s.
+  {idle_thread s, arm_globals_frame (arch_state s), arm_global_pd (arch_state s)} \<union>
+   range (interrupt_irq_node s) \<union>
+   set (arm_global_pts (arch_state s))"
+
+definition
+  kernel_window :: "'z::state_ext state \<Rightarrow> obj_ref set"
+where
+  "kernel_window s \<equiv> {x. arm_kernel_vspace (arch_state s) x \<noteq> ArmVSpaceKernelWindow}"
+
+
+  (* needed for map: installing new object should add only one mapping *)
+definition
+  "valid_table_caps \<equiv> \<lambda>s.
+  \<forall>r p acap. arch_caps_of_state s p = Some acap \<longrightarrow>
+            (is_pd_cap acap \<or> is_pt_cap acap) \<longrightarrow>
+            cap_asid acap = None \<longrightarrow>
+            aobj_ref acap = Some r \<longrightarrow>
+            aobj_at (empty_table (set (arm_global_pts (arch_state s)))) r s"
+
+  (* needed to preserve valid_table_caps in map *)
+definition
+  "unique_table_caps \<equiv> \<lambda>cs. \<forall>p p' cap cap'.
+  cs p = Some cap \<longrightarrow> cs p' = Some cap' \<longrightarrow>
+  cap_asid cap = None \<longrightarrow>
+  aobj_ref cap' = aobj_ref cap \<longrightarrow>
+  (is_pd_cap cap \<longrightarrow> is_pd_cap cap' \<longrightarrow> p' = p) \<and>
+  (is_pt_cap cap \<longrightarrow> is_pt_cap cap' \<longrightarrow> p' = p)"
+
+definition
+  table_cap_ref :: "arch_cap \<Rightarrow> vs_ref list option"
+where
+  "table_cap_ref cap \<equiv> case cap of
+     Arch_Structs_A.ASIDPoolCap _ asid \<Rightarrow>
+       Some [VSRef (ucast (asid_high_bits_of asid)) None]
+   | Arch_Structs_A.PageDirectoryCap _ (Some asid) \<Rightarrow>
+       Some [VSRef (asid && mask asid_low_bits) (Some AASIDPool),
+             VSRef (ucast (asid_high_bits_of asid)) None]
+   | Arch_Structs_A.PageTableCap _ (Some (asid, vptr)) \<Rightarrow>
+       Some [VSRef (vptr >> 20) (Some APageDirectory),
+             VSRef (asid && mask asid_low_bits) (Some AASIDPool),
+             VSRef (ucast (asid_high_bits_of asid)) None]
+   | _ \<Rightarrow> None"
+
+  (* needed to avoid a single page insertion
+     resulting in multiple valid lookups *)
+definition
+  "unique_table_refs \<equiv> \<lambda>cs. \<forall>p p' cap cap'.
+  cs p = Some cap \<longrightarrow> cs p' = Some cap' \<longrightarrow>
+  aobj_ref cap' = aobj_ref cap \<longrightarrow>
+  table_cap_ref cap' = table_cap_ref cap"
+
+definition
+  valid_kernel_mappings :: "'z::state_ext state \<Rightarrow> bool"
+where
+  "valid_kernel_mappings \<equiv>
+     \<lambda>s. \<forall>ko \<in> ran (kheap s).
+          valid_kernel_mappings_if_pd
+             (set (arm_global_pts (arch_state s))) ko"
+
+definition
+  "valid_arch_caps \<equiv> valid_vs_lookup and valid_table_caps and
+                     (\<lambda>s. unique_table_caps (arch_caps_of_state s)
+                        \<and> unique_table_refs (arch_caps_of_state s))"
+
+definition
+  "valid_machine_state \<equiv>
+   \<lambda>s. \<forall>p. in_user_frame p (s::'z::state_ext state) \<or> underlying_memory (machine_state s) p = 0"
+
+text "objects live in the kernel window"
+definition
+  pspace_in_kernel_window :: "'z::state_ext state \<Rightarrow> bool"
+where
+ "pspace_in_kernel_window \<equiv> \<lambda>s.
+    \<forall>x ko. kheap s x = Some ko \<longrightarrow>
+       (\<forall>y \<in> {x .. x + (2 ^ obj_bits ko) - 1}.
+             arm_kernel_vspace (arch_state s) y = ArmVSpaceKernelWindow)"
+
+definition
+  arch_obj_bits_type :: "aa_type \<Rightarrow> nat"
+where
+ "arch_obj_bits_type T' \<equiv> (case T' of
+    AASIDPool \<Rightarrow> arch_kobj_size (Arch_Structs_A.ASIDPool undefined)
+  | AIntData sz \<Rightarrow> arch_kobj_size (DataPage sz)
+  | APageDirectory \<Rightarrow> arch_kobj_size (Arch_Structs_A.PageDirectory undefined)
+  | APageTable \<Rightarrow> arch_kobj_size (Arch_Structs_A.PageTable undefined))"
+
+section "Lemmas"
+
+lemma vmsz_aligned_ARMSection:
+  "vmsz_aligned vref ARMSection = is_aligned vref (pageBitsForSize ARMSection)"
+  by (simp add: vmsz_aligned_def pageBitsForSize_def)
+
+lemma valid_arch_cap_def2:
+  "valid_arch_cap c s \<equiv> wellformed_acap c \<and> valid_arch_cap_ref c s"
+  apply (rule eq_reflection)
+  apply (cases c)
+    by (auto simp add: wellformed_acap_simps valid_arch_cap_simps
+                          valid_arch_cap_ref_simps vmsz_aligned_ARMSection
+                split: option.splits)
+
+lemmas vs_ref_atype_simps[simp] = vs_ref_atype_def[split_simps vs_ref.split]
+
+lemma vs_lookup1_obj_at:
+  "((rs,p) \<rhd>1 (r # rs,p')) s = aobj_at (\<lambda>ko. (r, p') \<in> vs_refs ko) p s"
+  by (fastforce simp: vs_lookup1_def aobj_at_def)
+
+lemma vs_lookup1I:
+  "\<lbrakk> ako_at ko p s; (r, p') \<in> vs_refs ko;
+          rs' = r # rs \<rbrakk> \<Longrightarrow> ((rs,p) \<rhd>1 (rs',p')) s"
+  by (fastforce simp add: vs_lookup1_def)
+
+lemma vs_lookup1D:
+  "(x \<rhd>1 y) s \<Longrightarrow> \<exists>rs r p p' ko. x = (rs,p) \<and> y = (r # rs,p')
+                          \<and> ako_at ko p s \<and> (r,p') \<in> vs_refs ko"
+  by (cases x, cases y) (fastforce simp: vs_lookup1_def)
+
+lemma vs_lookup_pages1D:
+  "(x \<unrhd>1 y) s \<Longrightarrow> \<exists>rs r p p' ko. x = (rs,p) \<and> y = (r # rs,p')
+                          \<and> ako_at ko p s \<and> (r,p') \<in> vs_refs_pages ko"
+  by (cases x, cases y) (fastforce simp: vs_lookup_pages1_def)
+
+lemma vs_lookup1_stateI:
+  assumes 1: "(r \<rhd>1 r') s"
+  assumes ko: "\<And>ko. ako_at ko (snd r) s \<Longrightarrow> aobj_at (\<lambda>ko'. vs_refs ko \<subseteq> vs_refs ko') (snd r) s'"
+  shows "(r \<rhd>1 r') s'" using 1 ko
+  by (fastforce simp: aobj_at_def vs_lookup1_def)
+
+lemma vs_lookup_trans_sub:
+  assumes ko: "\<And>ko p. ako_at ko p s \<Longrightarrow> aobj_at (\<lambda>ko'. vs_refs ko \<subseteq> vs_refs ko') p s'"
+  shows "vs_lookup_trans s \<subseteq> vs_lookup_trans s'"
+proof -
+  have "vs_lookup1 s \<subseteq> vs_lookup1 s'"
+    by (fastforce dest: ko elim: vs_lookup1_stateI)
+  thus ?thesis by (rule rtrancl_mono)
+qed
+
+lemma vs_lookup_sub:
+  assumes ko: "\<And>ko p. ako_at ko p s \<Longrightarrow> aobj_at (\<lambda>ko'. vs_refs ko \<subseteq> vs_refs ko') p s'"
+  assumes table: "graph_of (arm_asid_table (arch_state s)) \<subseteq> graph_of (arm_asid_table (arch_state s'))"
+  shows "vs_lookup s \<subseteq> vs_lookup s'"
+  unfolding vs_lookup_def
+  apply (rule Image_mono)
+   apply (rule vs_lookup_trans_sub)
+   apply (erule ko)
+  apply (unfold vs_asid_refs_def)
+  apply (rule image_mono)
+  apply (rule table)
+  done
+
+lemma vs_lookup_pages1_stateI:
+  assumes 1: "(r \<unrhd>1 r') s"
+  assumes ko: "\<And>ko. ako_at ko (snd r) s \<Longrightarrow> aobj_at (\<lambda>ko'. vs_refs_pages ko \<subseteq> vs_refs_pages ko') (snd r) s'"
+  shows "(r \<unrhd>1 r') s'" using 1 ko
+  by (fastforce simp: aobj_at_def vs_lookup_pages1_def)
+
+lemma vs_lookup_pages_trans_sub:
+  assumes ko: "\<And>ko p. ako_at ko p s \<Longrightarrow>
+                      aobj_at (\<lambda>ko'. vs_refs_pages ko \<subseteq> vs_refs_pages ko') p s'"
+  shows "vs_lookup_pages_trans s \<subseteq> vs_lookup_pages_trans s'"
+proof -
+  have "vs_lookup_pages1 s \<subseteq> vs_lookup_pages1 s'"
+    by (fastforce simp add: ko elim: vs_lookup_pages1_stateI)
+  thus ?thesis by (rule rtrancl_mono)
+qed
+
+lemma vs_lookup_pages_sub:
+  assumes ko: "\<And>ko p. ako_at ko p s \<Longrightarrow>
+                      aobj_at (\<lambda>ko'. vs_refs_pages ko \<subseteq> vs_refs_pages ko') p s'"
+  assumes table:
+    "graph_of (arm_asid_table (arch_state s)) \<subseteq>
+     graph_of (arm_asid_table (arch_state s'))"
+  shows "vs_lookup_pages s \<subseteq> vs_lookup_pages s'"
+  unfolding vs_lookup_pages_def
+  apply (rule Image_mono)
+   apply (rule vs_lookup_pages_trans_sub)
+   apply (erule ko)
+  apply (unfold vs_asid_refs_def)
+  apply (rule image_mono)
+  apply (rule table)
+  done
+
+lemma vs_lookup_pagesI:
+  "\<lbrakk> ref' \<in> vs_asid_refs (arm_asid_table (arch_state s));
+     (ref',(ref,p)) \<in> (vs_lookup_pages1 s)^*  \<rbrakk> \<Longrightarrow>
+  (ref \<unrhd> p) s"
+  by (simp add: vs_lookup_pages_def) blast
+
+lemma vs_lookup_stateI:
+  assumes 1: "(ref \<rhd> p) s"
+  assumes ko: "\<And>ko p. ako_at ko p s \<Longrightarrow> aobj_at (\<lambda>ko'. vs_refs ko \<subseteq> vs_refs ko') p s'"
+  assumes table: "graph_of (arm_asid_table (arch_state s)) \<subseteq> graph_of (arm_asid_table (arch_state s'))"
+  shows "(ref \<rhd> p) s'"
+  using 1 vs_lookup_sub [OF ko table] by blast
+
+lemma valid_arch_objsD:
+  "\<lbrakk> (ref \<rhd> p) s; ako_at ao p s; valid_arch_objs s \<rbrakk> \<Longrightarrow> valid_arch_obj ao s"
+  by (fastforce simp add: valid_arch_objs_def)
+
+(* should work for unmap and non-arch ops *)
+lemma valid_arch_objs_stateI:
+  assumes 1: "valid_arch_objs s"
+  assumes ko: "\<And>ko p. ako_at ko p s' \<Longrightarrow> aobj_at (\<lambda>ko'. vs_refs ko \<subseteq> vs_refs ko') p s"
+  assumes arch: "graph_of (arm_asid_table (arch_state s')) \<subseteq> graph_of (arm_asid_table (arch_state s))"
+  assumes vao: "\<And>p ref ao'.
+                \<lbrakk> (ref \<rhd> p) s; (ref \<rhd> p) s'; \<forall>ao. ako_at ao p s \<longrightarrow> valid_arch_obj ao s;
+                  ako_at ao' p s' \<rbrakk> \<Longrightarrow> valid_arch_obj ao' s'"
+  shows "valid_arch_objs s'"
+  using 1 unfolding valid_arch_objs_def
+  apply clarsimp
+  apply (frule vs_lookup_stateI)
+    apply (erule ko)
+   apply (rule arch)
+  apply (erule allE, erule impE, fastforce)
+  apply (erule (3) vao)
+  done
+
+lemma aobj_at_pspaceI:
+  "\<lbrakk> aobj_at P ref s; kheap s = kheap s' \<rbrakk> \<Longrightarrow> aobj_at P ref s'"
+  by (simp add: aobj_at_def)
+
+
+lemma valid_arch_cap_atyp:
+  assumes P: "\<And>P T p. \<lbrace>\<lambda>s. P (atyp_at T p s)\<rbrace> f \<lbrace>\<lambda>rv s. P (atyp_at T p s)\<rbrace>"
+  shows      "\<lbrace>\<lambda>s. valid_arch_cap c s\<rbrace> f \<lbrace>\<lambda>rv s. valid_arch_cap c s\<rbrace>"
+  apply (simp add: valid_arch_cap_def)
+  apply (case_tac c, simp_all)
+  by (wp P)
+
+lemma valid_arch_obj_atyp:
+  assumes P: "\<And>P p T. \<lbrace>\<lambda>s. P (atyp_at T p s)\<rbrace> f \<lbrace>\<lambda>rv s. P (atyp_at T p s)\<rbrace>"
+  shows      "\<lbrace>\<lambda>s. valid_arch_obj ob s\<rbrace> f \<lbrace>\<lambda>rv s. valid_arch_obj ob s\<rbrace>"
+  apply (cases ob, simp_all)
+     apply (rule hoare_vcg_const_Ball_lift [OF P])
+    apply (rule hoare_vcg_all_lift)
+    apply (rename_tac "fun" x)
+    apply (case_tac "fun x", simp_all add: hoare_vcg_prop P)
+  apply (rule hoare_vcg_ball_lift)
+  apply (rename_tac "fun" x)
+  apply (case_tac "fun x", simp_all add: hoare_vcg_prop P)
+  apply (rule P)
+  done
+
+lemma atyp_at_eq_kheap_obj:
+  "atyp_at AASIDPool p s \<longleftrightarrow>
+   (\<exists>f. kheap s p = Some (ArchObj (Arch_Structs_A.ASIDPool f)))"
+  "atyp_at APageTable p s \<longleftrightarrow>
+   (\<exists>pt. kheap s p = Some (ArchObj (PageTable pt)))"
+  "atyp_at APageDirectory p s \<longleftrightarrow>
+   (\<exists>pd. kheap s p = Some (ArchObj (PageDirectory pd)))"
+  "atyp_at (AIntData sz) p s \<longleftrightarrow>
+   (kheap s p = Some (ArchObj (DataPage sz)))"
+apply (auto simp add: aobj_at_def)
+apply (simp_all add: aa_type_def split: split_if_asm  arch_kernel_obj.splits)
+done
+
+lemma aa_type_AASIDPoolE:
+  "\<lbrakk>aa_type ko = AASIDPool;
+    (\<And>ap. ko = (arch_kernel_obj.ASIDPool ap) \<Longrightarrow> R)\<rbrakk>
+   \<Longrightarrow> R"
+  by (case_tac ko, simp_all add: aa_type_simps split: split_if_asm)
+
+lemma aa_type_APageDirectoryE:
+  "\<lbrakk>aa_type ko = APageDirectory;
+    (\<And>pd. ko = PageDirectory pd \<Longrightarrow> R)\<rbrakk>
+   \<Longrightarrow> R"
+  by (case_tac ko, simp_all add: aa_type_simps split: split_if_asm)
+
+lemma aa_type_APageTableE:
+  "\<lbrakk>aa_type ko = APageTable; (\<And>pt. ko = PageTable pt \<Longrightarrow> R)\<rbrakk>
+   \<Longrightarrow> R"
+  by (case_tac ko, simp_all add: aa_type_simps split: split_if_asm)
+
+lemma aa_type_AIntDataE:
+  "\<lbrakk>aa_type ko = AIntData sz; ko = DataPage sz \<Longrightarrow> R\<rbrakk> \<Longrightarrow> R"
+  by (case_tac ko, simp_all add: aa_type_simps split: split_if_asm)
+
+
+
+lemmas a_type_elims[elim!] =
+   aa_type_AASIDPoolE aa_type_APageDirectoryE aa_type_APageTableE aa_type_AIntDataE
+
+end
+
+end
