spec/abstract/ARM/ArchRetype_A.thy
@@ -20,6 +20,8 @@ imports
   ArchInvocation_A
 begin
 
+context ARM begin
+
 text {* This is a placeholder function. We may wish to extend the specification
   with explicitly tagging kernel data regions in memory. *}
 definition
@@ -58,5 +60,7 @@ where
                                                       (addrFromPPtr x)) refs
     od
   | _ \<Rightarrow> return ()"
+
+end
 
 end
