spec/abstract/Interrupt_A.thy
@@ -18,6 +18,9 @@ theory Interrupt_A
 imports Ipc_A
 begin
 
+unqualify_consts (in "$L4V_ARCH")
+  "arch_invoke_irq_control :: arch_irq_control_invocation \<Rightarrow> (unit,'z::state_ext) p_monad"
+  setInterruptMode
 text {* Tests whether an IRQ identifier is in use. *}
 definition
   is_irq_active :: "irq \<Rightarrow> (bool,'z::state_ext) s_monad" where
