spec/abstract/InvocationLabels_A.thy
@@ -20,6 +20,12 @@ imports
   "../design/$L4V_ARCH/ArchLabelFuns_H"
 begin
 
+unqualify_types (in "$L4V_ARCH") 
+  data
+
+unqualify_consts (in "$L4V_ARCH") 
+  "data_to_nat :: data \<Rightarrow> nat"
+
 definition
   invocation_type :: "data \<Rightarrow> invocation_label"
 where
