spec/abstract/Ipc_A.thy
@@ -18,6 +18,10 @@ theory Ipc_A
 imports Tcb_A
 begin
 
+unqualify_consts (in "$L4V_ARCH")
+  "set_message_info :: obj_ref \<Rightarrow> message_info \<Rightarrow> (unit,'z::state_ext) s_monad"
+  "lookup_ipc_buffer :: bool \<Rightarrow> obj_ref \<Rightarrow> (obj_ref option,'z::state_ext) s_monad"
+
 section {* Getting and setting the message info register. *}
 
 definition
