spec/abstract/Retype_A.thy
@@ -22,6 +22,12 @@ imports
   "./$L4V_ARCH/ArchRetype_A"
 begin
 
+unqualify_consts (in "$L4V_ARCH")
+  "arch_default_cap :: aobject_type \<Rightarrow> obj_ref \<Rightarrow> nat \<Rightarrow> arch_cap"
+  "default_arch_object :: aobject_type \<Rightarrow> nat \<Rightarrow> arch_kernel_obj"
+  "init_arch_objects :: apiobject_type \<Rightarrow> obj_ref \<Rightarrow> nat \<Rightarrow> nat \<Rightarrow> obj_ref list \<Rightarrow> (unit,'z::state_ext) s_monad"
+
+
 section "Creating Caps"
 
 text {* The original capability created when an object of a given type is
