spec/abstract/TcbAcc_A.thy
@@ -18,6 +18,9 @@ theory TcbAcc_A
 imports CSpace_A
 begin
 
+unqualify_consts (in "$L4V_ARCH")
+  "in_user_frame :: obj_ref \<Rightarrow> 'z::state_ext state \<Rightarrow> bool"
+
 text {* Store or load a word at an offset from an IPC buffer. *}
 definition
   store_word_offs :: "obj_ref \<Rightarrow> nat \<Rightarrow> machine_word \<Rightarrow> (unit,'z::state_ext) s_monad" where
