spec/abstract/Tcb_A.thy
@@ -18,6 +18,9 @@ theory Tcb_A
 imports TcbAcc_A Schedule_A
 begin
 
+unqualify_consts (in "$L4V_ARCH")
+  "arch_activate_idle_thread :: obj_ref \<Rightarrow> (unit,'z::state_ext) s_monad"
+
 section "Activating Threads"
 
 text {* Threads that are active always have a master Reply capability to
