spec/design/ARM/ArchLabelFuns_H.thy
@@ -14,6 +14,8 @@ theory ArchLabelFuns_H
 imports "../InvocationLabels_H"
 begin
 
+context ARM begin
+
 text {*
   Arch-specific functions on invocation labels
 *}
@@ -39,6 +41,6 @@ where
       | ArchInvocationLabel ARMPageUnify_Instruction \<Rightarrow>   True
       | _ \<Rightarrow>   False
       )"
-
+end
 
 end
