spec/machine/MachineExports.thy
@@ -1,0 +1,40 @@
+(*
+ * Copyright 2014, General Dynamics C4 Systems
+ *
+ * This software may be distributed and modified according to the terms of
+ * the GNU General Public License version 2. Note that NO WARRANTY is provided.
+ * See "LICENSE_GPLv2.txt" for details.
+ *
+ * @TAG(GD_GPL)
+ *)
+
+
+theory MachineExports
+imports "./$L4V_ARCH/MachineOps"
+begin
+  
+unqualify_types (in "$L4V_ARCH")
+  machine_word 
+  vmfault_type
+  irq
+
+unqualify_consts (in "$L4V_ARCH")
+  "getActiveIRQ :: (irq option) machine_monad"
+  "maskInterrupt :: bool \<Rightarrow> irq \<Rightarrow> unit machine_monad"
+  "freeMemory :: machine_word \<Rightarrow> nat \<Rightarrow> unit machine_monad"
+  "loadWord :: machine_word \<Rightarrow> machine_word machine_monad"
+  "storeWord :: machine_word \<Rightarrow> machine_word \<Rightarrow> unit machine_monad"
+  "storeWordVM :: machine_word \<Rightarrow> machine_word \<Rightarrow> unit machine_monad"
+  "setNextPC :: machine_word \<Rightarrow> unit user_monad"
+  "getRestartPC :: machine_word user_monad"
+  "setRegister :: register \<Rightarrow> machine_word \<Rightarrow> unit user_monad"
+  "getRegister :: register \<Rightarrow> machine_word user_monad"
+  "sanitiseRegister :: register \<Rightarrow> machine_word \<Rightarrow> machine_word"
+  "initContext :: (register * machine_word) list"
+  "exceptionMessage :: register list"
+  "syscallMessage :: register list"
+  "gpRegisters :: register list"
+  "frameRegisters :: register list"
+  "setInterruptMode :: irq \<Rightarrow> bool \<Rightarrow> bool \<Rightarrow> unit machine_monad"
+
+end
