spec/machine/MachineMonad.thy
@@ -1,0 +1,93 @@
+(*
+ * Copyright 2014, General Dynamics C4 Systems
+ *
+ * This software may be distributed and modified according to the terms of
+ * the GNU General Public License version 2. Note that NO WARRANTY is provided.
+ * See "LICENSE_GPLv2.txt" for details.
+ *
+ * @TAG(GD_GPL)
+ *)
+
+
+theory MachineMonad
+imports "./$L4V_ARCH/MachineTypes"
+begin
+  
+unqualify_types (in "$L4V_ARCH")
+  machine_state
+  machine_state_rest
+
+unqualify_consts (in "$L4V_ARCH")
+  "machine_state_rest :: machine_state \<Rightarrow> machine_state_rest"
+  "machine_state_rest_update :: (machine_state_rest \<Rightarrow> machine_state_rest) \<Rightarrow> machine_state \<Rightarrow> machine_state"
+
+text {*
+  The machine monad is used for operations on the state defined above.
+*}
+type_synonym 'a machine_monad = "(machine_state, 'a) nondet_monad"
+
+translations
+  (type) "'c machine_monad" <= (type) "(machine_state, 'c) nondet_monad"
+
+type_synonym 'a machine_rest_monad = "(machine_state_rest, 'a) nondet_monad"
+
+definition
+  machine_rest_lift :: "'a machine_rest_monad \<Rightarrow> 'a machine_monad"
+where
+  "machine_rest_lift f \<equiv> do
+    mr \<leftarrow> gets machine_state_rest;
+    (r, mr') \<leftarrow> select_f (f mr);
+    modify (\<lambda>s. s \<lparr> machine_state_rest := mr' \<rparr>);
+    return r
+  od"
+
+
+definition
+  ignore_failure :: "('s,unit) nondet_monad \<Rightarrow> ('s,unit) nondet_monad"
+  where 
+  "ignore_failure f \<equiv> 
+  \<lambda>s. if fst (f s) = {} then ({((),s)},False) else (fst (f s), False)"
+
+text {* The wrapper doesn't do anything for usual operations: *}
+lemma failure_consistent:
+  "\<lbrakk> empty_fail f; no_fail \<top> f \<rbrakk> \<Longrightarrow> ignore_failure f = f"
+  apply (simp add: ignore_failure_def empty_fail_def no_fail_def)
+  apply (rule ext)
+  apply (auto intro: prod_eqI)
+  done
+  
+text {* And it has the desired properties *}
+lemma ef_ignore_failure [simp]:
+  "empty_fail (ignore_failure f)"
+  by (simp add: empty_fail_def ignore_failure_def)
+
+lemma no_fail_ignore_failure [simp, intro!]:
+  "no_fail \<top> (ignore_failure f)"
+  by (simp add: no_fail_def ignore_failure_def)
+
+
+lemma ef_machine_rest_lift [simp, intro!]:
+  "empty_fail f \<Longrightarrow> empty_fail (machine_rest_lift f)"
+  apply (clarsimp simp: empty_fail_def machine_rest_lift_def simpler_gets_def 
+                        select_f_def bind_def simpler_modify_def return_def)
+  apply force
+  done
+    
+lemma no_fail_machine_state_rest [intro!]:
+  "no_fail P f \<Longrightarrow> no_fail (P o machine_state_rest) (machine_rest_lift f)"
+  apply (simp add: no_fail_def machine_rest_lift_def simpler_gets_def 
+                        select_f_def bind_def simpler_modify_def return_def)
+  apply force
+  done
+ 
+lemma no_fail_machine_state_rest_T [simp, intro!]:
+  "no_fail \<top> f \<Longrightarrow> no_fail \<top> (machine_rest_lift f)"
+  apply (drule no_fail_machine_state_rest)
+  apply (simp add: o_def)
+  done
+
+definition
+  "machine_op_lift \<equiv> machine_rest_lift o ignore_failure"
+
+
+end
